setting up interface

Examples/SystemFWithNat/Term.lean
@@ -1,5 +1,7 @@
 
 import LeanSubst
+import LeanSubst.Automation.Attributes
+
 open LeanSubst
 
 namespace SystemFWithNat
@@ -15,11 +17,23 @@ inductive Term where
 | app : Term -> Term -> Term
 | lam (A : Ty) (t : Term) : Term -- binds Term in t
 | tapp : Term -> Ty -> Term
-
 | tlam (t : Term) : Term -- binds Ty in t (does it make sense to allow a user to give a name instead of a position?)
 | zero : Term
 | succ : Term -> Term
 | nrec (motive : Ty) (z : Term) (s : Term) (n : Term) : Term -- binds 2 Term's in s
+
+#leansubst var Ty.var
+#leansubst bind Ty at pos 0 in Ty.all
+
+#eval do
+  pure (LeanSubstAttributes.leanSubstBinder.getParam? (← Lean.MonadEnv.getEnv) ``Ty.all)
+
+#leansubst var Term.var
+#leansubst bind Term at pos 1 in Term.lam
+#leansubst bind Ty at pos 0 in Term.tlam
+#leansubst bind
+  2 of Term at pos 2
+  in Term.nrec
 
 /-
 
@@ -53,19 +67,19 @@ instance : SubstMap Ty [Ty] where
 
 @[coe]
 def Term.from_action : Action Term -> Term
-| re y => var y
+| re y => .var y
 | su t => t
 
 @[simp, grind =]
-theorem Term.from_action_id {n} : from_action (𝐬0.act n) = var n := by
+theorem Term.from_action_id {n} : from_action (𝐬0.act n) = .var n := by
   simp [from_action]
 
 @[simp, grind =]
-theorem Term.from_action_succ {n} : from_action (𝐬1.act n) = var (n + 1) := by
+theorem Term.from_action_succ {n} : from_action (𝐬1.act n) = .var (n + 1) := by
   simp [from_action]
 
 @[simp, grind =]
-theorem Term.from_acton_re {n} : from_action (re n) = var n := by simp [from_action]
+theorem Term.from_acton_re {n} : from_action (re n) = .var n := by simp [from_action]
 
 @[simp, grind =]
 theorem Term.from_action_su {t} : from_action (su t) = t := by simp [from_action]
@@ -76,7 +90,7 @@ instance : Coe (Action Term) Term where
 -- Defining the rmap/smap using the Tuple form might make more sense for a macro, dunno
 @[simp]
 def Term.rmap (r : RenVec [Term, Ty]) : Term -> Term
-| var x => var (r.1.act x)
+| .var x => .var (r.1.act x)
 | app t1 t2 => app (t1.rmap r) (t2.rmap r)
 | lam A t => lam A⟨r.2.1⟩ (t.rmap $ r.lift [1, 0])
 | tapp t A => tapp (t.rmap r) A⟨r.2.1⟩
@@ -96,7 +110,7 @@ instance : RenMap Term [Ty] where
 
 @[simp]
 def Term.smap (σ : Subst Term) (τ : Subst Ty) : Term -> Term
-| var x => σ.act x
+| .var x => σ.act x
 | app t1 t2 => app (t1.smap σ τ) (t2.smap σ τ)
 | lam A t => lam A[τ] (t.smap σ.lift τ)
 | tapp t A => tapp (t.smap σ τ) A[τ]
