LeanSubst/Automation/Attributes.lean
@@ -1,55 +1,82 @@
 import Batteries.Lean.TagAttribute
-import Lean.Parser.Term
 import Lean.Elab
 
-open Lean Elab Tactic Meta Command
+namespace LeanSubstAttributes
 
-initialize leanSubstVar : TagAttribute ← registerTagAttribute `leansubst_var "Indicates that a constructor is a variable constructor."
+  open Lean Elab Tactic Meta Command
 
-#check Lean.Parser.Command.classAbbrev
-#check Lean.Parser.Term.attrInstance
-#check Attr.coe
+  initialize leanSubstVar : TagAttribute ← registerTagAttribute `leansubst_var "Indicates that a constructor is a variable constructor."
 
-#check Lean.Parser.Attr.simple
+  #check Lean.Parser.Command.classAbbrev
+  #check Lean.Parser.Term.attrInstance
+  #check Attr.coe
 
-#check mkElabAttribute
+  #check Lean.Parser.Attr.simple
 
-syntax (name := leansubst_binder_attr) "leansubst_binder" "(" term "," num "," term ")" : attr
+  #check mkElabAttribute
 
-initialize leanSubstBinder : ParametricAttribute (Term × Nat × Term) ← registerParametricAttribute {
-  name := `leansubst_binder_attr,
-  descr := "Blah",
-  getParam := fun
-  | name, stx@`(attr| leansubst_binder ($ty, $pos, $nBnd)) => do
-    dbg_trace s!"ty: {ty}"
-    dbg_trace s!"inArg: {pos}"
-    dbg_trace s!"nBnd: {nBnd}"
-    pure (ty, pos.getNat, nBnd)
-  | _, _ => throwUnsupportedSyntax
-}
+  declare_syntax_cat leansubst_attr
 
-initialize leanSubstBinder' : ParametricAttribute Nat ← registerParametricAttribute {
-  name := `leansubst_binder',
-  descr := "Blah",
-  getParam := fun
-  | name, stx@`(Lean.Parser.Attr.simple| $_ $n:num) => do
-    pure n.getNat
-  | name, stx@`(Lean.Parser.Term.attrInstance| $_) => do
-    dbg_trace s!"aw fuck {name}, {stx}"
-    pure 0
-}
+  syntax "(" term "," term "," num ")" : leansubst_attr
 
-elab "#leansubst" "bind" nBndClosure:term "of" ty:term "in" ctor:ident "at" "pos" pos:num : command => do
-  let nBndClosure ← match nBndClosure with
-  | `($n:num) => `(fun _ => $n)
-  | closure => pure closure
-  elabCommand $ ← `(
-    attribute [leansubst_binder ($ty, $pos, $nBndClosure)] $ctor
-  )
+  syntax (name := leansubst_binder_attr) "leansubst_binder" "[" term,* "]" "[" term,* "]" "[" num,* "]" : attr
 
-elab "#leansubst" "var" ctor:ident : command => do
-  elabCommand $ ← `(
-    attribute [leansubst_var] $ctor
-  )
+  initialize leanSubstBinder : ParametricAttribute $ List (Term × Term × Nat) ← registerParametricAttribute {
+    name := `leansubst_binder_attr,
+    descr := "Blah",
+    getParam := fun
+    | name, stx@`(attr| leansubst_binder [ $closures,* ] [ $tys,* ] [ $ps,* ]) => do
+      let ret := Array.zip closures.getElems (Array.zip tys.getElems ps.getElems)
+      pure $ ret.toList.map (fun (a, b, c) => (a, b, c.getNat))
+    | _, _ => throwUnsupportedSyntax
+  }
 
-elab "#leansubst" "generate" : command => sorry
+  initialize leanSubstBinder' : ParametricAttribute Nat ← registerParametricAttribute {
+    name := `leansubst_binder',
+    descr := "Blah",
+    getParam := fun
+    | name, stx@`(Lean.Parser.Attr.simple| $_ $n:num) => do
+      pure n.getNat
+    | name, stx@`(Lean.Parser.Term.attrInstance| $_) => do
+      dbg_trace s!"aw fuck {name}, {stx}"
+      pure 0
+  }
+
+  declare_syntax_cat bind_data
+
+  syntax term " of " term " at " " pos " num : bind_data
+
+  syntax term " at " " pos " num : bind_data
+
+  macro ty:term " at " " pos " p:num : bind_data => `(bind_data| 1 of $ty at pos $p)
+
+  declare_syntax_cat bind_decl
+
+  syntax " bind " bind_data,+ " in " ident : bind_decl
+
+  elab "#leansubst" stx:bind_decl : command => stx |> fun
+  | `(bind_decl| bind $data,* in $ctor) => do
+    let mapfun := fun
+    | `(bind_data| $closure:term of $ty:term at pos $p) => pure (closure, ty, p)
+    | `(bind_data| $ty:term at pos $p) => pure (Syntax.mkNatLit 1, ty, p) -- I thought the macros would be expanded, but this seems necessary
+    | _ => throwUnsupportedSyntax
+    let data ← data.getElems.mapM mapfun
+    let closures := data.map (·.1)
+    let tys := data.map (·.2.1)
+    let ps : Array (TSyntax `num) := data.map (·.2.2)
+    dbg_trace "Elabbing command"
+    elabCommand $ ← `(
+      attribute [leansubst_binder [$closures,*] [$tys,*] [$ps,*]] $ctor
+    )
+    dbg_trace "Done!"
+  | _ => throwUnsupportedSyntax
+
+
+  elab "#leansubst" "var" ctor:ident : command => do
+    elabCommand $ ← `(
+      attribute [leansubst_var] $ctor
+    )
+
+  elab "#leansubst" "generate" : command => sorry
+
+end LeanSubstAttributes
