LeanSubst/Automation/Basic.lean
@@ -7,29 +7,6 @@ import Aesop
 namespace Automation
   open Lean Elab Tactic Meta LeanSubst Command Aesop
 
-  def r1 : Ren Nat := sorry
-  def r2 : Ren Bool := sorry
-
-  #eval do
-    let stx1 ← ``(r1)
-    let stx2 ← ``(r2)
-
-    let ⟨expr1, _⟩ ← Term.TermElabM.run $ Term.elabTerm stx1 none
-    let ⟨expr2, _⟩ ← Term.TermElabM.run $ Term.elabTerm stx2 none
-
-    let type1 ← inferType expr1
-    let type2 ← inferType expr2
-
-    let type1' := match type1 with
-    | .app _ ty => some ty
-    | _ => none
-    let type2' := match type2 with
-    | .app _ ty => some ty
-    | _ => none
-
-    dbg_trace s!"{[type1', type2']}"
-
-
   def getConstructors (typeName : Name) : MetaM (List Name) := do
     match (← getEnv).find? typeName with
     | some (.inductInfo val) => return val.ctors
